HOL_To_IMP_Minus/Refinements/HOL_To_IMP_Minus_Lists.thy
@@ -173,6 +173,19 @@ case_of_simps map_acc_eq : map_acc.simps
 lemma map_eq_map_acc_nil: "map f xs = map_acc f xs []"
   by (simp add: map_acc_eq_rev_append_map)
 
+fun filter_acc :: "('a \<Rightarrow> bool) \<Rightarrow> 'a list \<Rightarrow> 'a list \<Rightarrow> 'a list"  where
+  "filter_acc p [] acc = rev acc"
+| "filter_acc p (x#xs) acc = filter_acc p xs (case p x of True \<Rightarrow> x # acc | False \<Rightarrow> acc)"
+declare filter_acc.simps[simp del]
+
+lemma filter_acc_eq_rev_append_map: "filter_acc p xs acc = rev acc @ filter p xs"
+  by (induction xs arbitrary: acc) (simp_all add: filter_acc.simps)
+
+case_of_simps filter_acc_eq : filter_acc.simps
+
+lemma filter_eq_filter_acc_nil: "filter p xs = filter_acc p xs []"
+  by (simp add: filter_acc_eq_rev_append_map)
+
 fun enumerate_acc :: "nat \<Rightarrow> 'a list \<Rightarrow> (nat \<times> 'a) list \<Rightarrow> (nat \<times> 'a) list"  where
   "enumerate_acc i [] acc = rev acc"
 | "enumerate_acc i (x#xs) acc = enumerate_acc (Suc i) xs ((i, x) # acc)"
@@ -201,6 +214,180 @@ HOL_To_IMP_Minus_correct HOL_To_HOL_Nat.enumerate_acc_nat by cook
 
 compile_nat HTHN.enumerate_nat_eq_unfolded
 HOL_To_IMP_Minus_correct HOL_To_HOL_Nat.enumerate_nat by cook
+
+end
+
+context HOL_To_HOL_Nat
+begin
+
+definition "map_pair_acc x = map_acc (Pair x)"
+lemmas map_pair_acc_eq = map_acc_eq[of "Pair x" for x, folded map_pair_acc_def]
+function_compile_nat map_pair_acc_eq
+
+fun product_acc :: "'a list \<Rightarrow> 'b list \<Rightarrow> ('a \<times> 'b) list \<Rightarrow> ('a \<times> 'b) list"  where
+  "product_acc [] _ acc = acc"
+| "product_acc (x#xs) ys acc =  product_acc xs ys (acc @ map_pair_acc x ys [])"
+declare product_acc.simps[simp del]
+
+lemma product_acc_eq_append_product: "product_acc xs ys acc = acc @ List.product xs ys"
+  by (induction xs arbitrary: acc)
+    (simp_all add: product_acc.simps map_pair_acc_def map_eq_map_acc_nil)
+
+case_of_simps product_acc_eq : product_acc.simps
+function_compile_nat product_acc_eq
+
+lemma product_eq_product_acc_nil: "List.product xs ys = product_acc xs ys []"
+  by (simp add: product_acc_eq_append_product)
+
+function_compile_nat product_eq_product_acc_nil
+
+end
+
+context HOL_Nat_To_IMP_Minus
+begin
+
+lemmas map_pair_acc_nat_eq = HTHN.map_pair_acc_nat_eq_unfolded[simplified case_list_nat_def]
+compile_nat map_pair_acc_nat_eq
+HOL_To_IMP_Minus_correct HOL_To_HOL_Nat.map_pair_acc_nat
+  apply (tactic \<open>HM.correct_if_IMP_tailcall_correct_tac HT.get_IMP_def @{context} 1\<close>)
+  by (induction "Pair y :: 'b \<Rightarrow> _" _ _ arbitrary: s rule: HOL_To_HOL_Nat.map_acc.induct)
+  (tactic \<open>HT.start_run_finish_case_tac HT.get_IMP_def HT.get_imp_minus_correct
+    HB.get_HOL_eqs @{context} 1\<close>)+
+
+lemmas product_acc_nat_eq = HTHN.product_acc_nat_eq_unfolded[simplified case_list_nat_def]
+compile_nat product_acc_nat_eq
+HOL_To_IMP_Minus_correct HOL_To_HOL_Nat.product_acc_nat by cook
+
+lemmas product_nat_eq = HTHN.product_nat_eq_unfolded[simplified case_list_nat_def]
+compile_nat product_nat_eq
+HOL_To_IMP_Minus_correct HOL_To_HOL_Nat.product_nat by cook
+
+end
+
+context HOL_To_HOL_Nat
+begin
+
+fun concat_acc :: "'a list list \<Rightarrow> 'a list \<Rightarrow> 'a list"  where
+  "concat_acc [] acc = acc"
+| "concat_acc (x#xs) acc = concat_acc xs (acc @ x)"
+declare concat_acc.simps[simp del]
+
+lemma concat_acc_eq_append_concat: "concat_acc xs acc = acc @ concat xs"
+  by (induction xs arbitrary: acc) (simp_all add: concat_acc.simps)
+
+case_of_simps concat_acc_eq : concat_acc.simps
+function_compile_nat concat_acc_eq
+
+lemma concat_eq_concat_acc_nil: "concat xs = concat_acc xs []"
+  by (simp add: concat_acc_eq_append_concat)
+function_compile_nat concat_eq_concat_acc_nil
+
+end
+
+context HOL_Nat_To_IMP_Minus
+begin
+
+lemmas concat_acc_nat_eq = HTHN.concat_acc_nat_eq_unfolded[simplified case_list_nat_def]
+compile_nat concat_acc_nat_eq
+HOL_To_IMP_Minus_correct HOL_To_HOL_Nat.concat_acc_nat by (cook mode = induction)
+
+lemmas concat_nat_eq = HTHN.concat_nat_eq_unfolded
+compile_nat concat_nat_eq
+HOL_To_IMP_Minus_correct HOL_To_HOL_Nat.concat_nat by cook
+
+end
+
+context HOL_To_HOL_Nat
+begin
+
+fun ListMem' :: "'a \<Rightarrow> 'a list \<Rightarrow> bool"  where
+  "ListMem' a [] = False"
+| "ListMem' a (x#xs) = (if a = x then True else ListMem' a xs)"
+declare ListMem'.simps[simp del]
+
+lemma ListMem'_eq_ListMem: "ListMem' x ys = ListMem x ys"
+  by (induction ys) (simp_all add: ListMem'.simps ListMem_iff)
+
+case_of_simps ListMem_eq[unfolded ListMem'_eq_ListMem] : ListMem'.simps
+function_compile_nat ListMem_eq
+
+end
+
+context HOL_Nat_To_IMP_Minus
+begin
+
+lemmas ListMem_nat_eq = HTHN.ListMem_nat_eq_unfolded[simplified case_list_nat_def]
+compile_nat ListMem_nat_eq
+HOL_To_IMP_Minus_correct HOL_To_HOL_Nat.ListMem_nat
+  apply (tactic \<open>HM.correct_if_IMP_tailcall_correct_tac HT.get_IMP_def @{context} 1\<close>)
+  by (induction ya arbitrary: s)
+    (tactic \<open>HT.start_run_finish_case_tac HT.get_IMP_def HT.get_imp_minus_correct
+    HB.get_HOL_eqs @{context} 1\<close>)+
+
+end
+
+context HOL_To_HOL_Nat
+begin
+
+fun remdups_acc :: "'a list \<Rightarrow> 'a list \<Rightarrow> 'a list"  where
+  "remdups_acc [] acc = rev acc"
+| "remdups_acc (x#xs) acc = remdups_acc xs (case ListMem x xs of True \<Rightarrow> acc | False \<Rightarrow> (x # acc))"
+declare remdups_acc.simps[simp del]
+
+lemma remdups_acc_eq_rev_append_remdups: "remdups_acc xs acc = rev acc @ remdups xs"
+  by (induction xs arbitrary: acc) (simp_all add: remdups_acc.simps ListMem_iff)
+
+case_of_simps remdups_acc_eq : remdups_acc.simps
+function_compile_nat remdups_acc_eq
+
+lemma remdups_eq_remdups_acc_nil: "remdups xs = remdups_acc xs []"
+  by (simp add: remdups_acc_eq_rev_append_remdups)
+function_compile_nat remdups_eq_remdups_acc_nil
+
+end
+
+context HOL_Nat_To_IMP_Minus
+begin
+
+lemmas remdups_acc_nat_eq = HTHN.remdups_acc_nat_eq_unfolded[simplified case_list_nat_def case_bool_nat_def]
+compile_nat remdups_acc_nat_eq
+HOL_To_IMP_Minus_correct HOL_To_HOL_Nat.remdups_acc_nat
+  apply (tactic \<open>HM.correct_if_IMP_tailcall_correct_tac HT.get_IMP_def @{context} 1\<close>)
+  apply (induction y ya arbitrary: s rule: HTHN.remdups_acc.induct)
+  subgoal by  (tactic \<open>HT.start_run_finish_case_tac HT.get_IMP_def HT.get_imp_minus_correct
+    HB.get_HOL_eqs @{context} 1\<close>)
+  subgoal for x xs acc s
+    apply (cases "ListMem x xs")
+    apply (tactic \<open>HT.start_case_tac HT.get_IMP_def @{context} 1\<close>)
+    apply (tactic \<open>HT.run_step_tac HT.get_imp_minus_correct @{context} 1\<close>)+
+    apply (tactic \<open>HT.run_step_tac HT.get_imp_minus_correct @{context} 2\<close>)+
+    apply (tactic \<open>HT.run_HOL_fun_tac HB.get_HOL_eqs @{context} 1\<close>)
+    apply (tactic \<open>HT.run_HOL_fun_tac HB.get_HOL_eqs @{context} 2\<close>)
+    apply auto
+    apply (tactic \<open>HT.finish_tail_tac @{context} 1\<close>)
+    apply (tactic \<open>HT.finish_tail_tac @{context} 2\<close>)+
+    apply (smt (verit) False_nat_eq_zero HOL_To_HOL_Nat.ListMem_nat_eq_unfolded HOL_To_HOL_Nat.Rel_nat_ListMem_nat_unfolded
+        Rel_nat_selector_list(1,2) rewrite_ne_zero_if_Rel_nat)+
+    done
+done
+
+lemmas remdups_nat_eq = HTHN.remdups_nat_eq_unfolded
+compile_nat remdups_nat_eq
+HOL_To_IMP_Minus_correct HOL_To_HOL_Nat.remdups_nat by cook
+
+end
+
+context HOL_To_HOL_Nat
+begin
+
+fun list_all' :: "('a \<Rightarrow> bool) \<Rightarrow> 'a list \<Rightarrow> bool"  where
+  "list_all' p [] = True"
+| "list_all' p (x#xs) = (case p x of True \<Rightarrow> list_all' p xs | False \<Rightarrow> False)"
+
+lemma list_all'_eq_list_all: "list_all' p xs = list_all p xs"
+  by (induction xs) (simp_all split: bool.split)
+
+case_of_simps list_all_eq[unfolded list_all'_eq_list_all] : list_all'.simps
 
 end
 
